

Introduction to Analysis I HW7

B13902024 張沂魁

November 5, 2025

Problem 0.0.1 (15pts). Assume that (S, d) is a metric space, and let $f_n, f : S \rightarrow \mathbb{R}$ be real-valued functions. Suppose that $f_n \rightarrow f$ uniformly on S , and there exists a constant $M > 0$ such that

$$|f_n(x)| \leq M \quad \text{for all } x \in S \text{ and all } n.$$

Let $g : \overline{B(0; M)} \rightarrow \mathbb{R}$ be continuous, where

$$B(0; M) = \{y \in \mathbb{R} : |y| < M\}.$$

Define

$$h_n(x) = g(f_n(x)), \quad h(x) = g(f(x)), \quad x \in S.$$

Prove that $h_n \rightarrow h$ uniformly on S .

Proof. Since g is continuous, so for all $\varepsilon > 0$, there exists $\delta > 0$ s.t. $|x_1 - x_2| < \delta$ implies $|g(x_1) - g(x_2)| < \varepsilon$. Also, since $f_n \rightarrow f$ uniformly, so $\exists N' > 0$ s.t. $n \geq N'$ implies $|f_n(x) - f(x)| < \delta$ for all $x \in S$. Hence, we can pick $N = N'$ so that if $n \geq N$, then $|f_n(x) - f(x)| < \delta$ for all $x \in S$ and thus

$$|g(f_n(x)) - g(f(x))| < \varepsilon$$

for all $x \in S$, so we know $h_n \rightarrow h$ uniformly on S . ■

Problem 0.0.2 (15pts). Let $f_n(x) = x^n$. The sequence $\{f_n\}$ converges pointwise but not uniformly on $[0, 1]$. Let g be continuous on $[0, 1]$ with $g(1) = 0$. Prove that the sequence $\{g(x)x^n\}$ converges uniformly on $[0, 1]$.

Problem 0.0.3 (15pts). Assume that $g_{n+1}(x) \leq g_n(x)$ for each x in T and each $n = 1, 2, \dots$, and suppose that $g_n \rightarrow 0$ uniformly on T . Prove that

$$\sum (-1)^{n+1} g_n(x)$$

converges uniformly on T .

Proof. We first give a claim:

Claim 0.0.1. $g_n(x) \geq 0$ for all $x \in T$ and $n \in \mathbb{N}$.

Proof. If $-c = g_{n_1}(x_1) < 0$ for some $x_1 \in T$ and $n_1 \in \mathbb{N}$, then for all $n \geq n_1$ we have $g_n(x_1) \leq -c$. If we pick some ε s.t. $0 < \varepsilon < c$, then since $g_n \rightarrow 0$ uniformly on T , so there exists $N > 0$ s.t. $n \geq N$ implies $|g_n(x)| < \varepsilon < c$ for all $x \in T$, and thus if we pick $n_2 = \max\{N, n_1\}$, we know $g_{n_2}(x_1) \leq -c$ and thus $|g_{n_2}(x_1)| \geq c > \varepsilon$, which is a contradiction. ⊗

Now we define $S_n(x) = \sum_{k=1}^n (-1)^{k+1} g_k(x)$. We first show that

$$\lim_{n \rightarrow \infty} S_n = \sum_{k=1}^{\infty} (-1)^{k+1} g_k(x)$$

exists.

Claim 0.0.2. $0 \leq \sum_{k=n}^m (-1)^{k+1} g_k(x) \leq g_n(x)$ for all $n, m \in \mathbb{N}$ and $x \in T$.

Proof. If $m < n$, then $\sum_{k=n}^m (-1)^{k+1} g_k(x) = 0$, so it is true. If $m \geq n$, then note that

$$\begin{aligned} \sum_{k=n}^m (-1)^{k+1} g_k(x) &= g_n(x) - g_{n+1}(x) + \cdots + (-1)^m g_m(x) \\ &= g_n(x) - (g_{n+1}(x) - g_{n+2}(x)) - \cdots \leq g_n(x) \end{aligned}$$

since $g_i(x) - g_{i+1}(x) \geq 0$. Also, we can check that

$$\begin{aligned} \sum_{k=n}^m (-1)^{k+1} g_k(x) &= g_n(x) - g_{n+1}(x) + \cdots + (-1)^m g_m(x) \\ &= (g_n(x) - g_{n+1}(x)) + (g_{n+2}(x) - g_{n+3}(x)) + \cdots \geq 0, \end{aligned}$$

so we're done. \oplus

Now by [Claim 0.0.2](#) we know S_n is bounded for all $n \in \mathbb{N}$, and if we fix $x_0 \in T$ and suppose

$$a_k := S_{2k-1}(x_0), \quad b_k := S_{2k}(x_0),$$

then we can check $(a_k)_{k=1}^\infty$ is decreasing and $(b_k)_{k=1}^\infty$ is increasing, so they are both convergent since they are monotonic and bounded. Also, we know $(|a_k - b_k|)_{k=0}^\infty$ converges to 0 since

$$|a_k - b_k| = |(-1)^{2k} g_{2k}(x_0)| = g_{2k}(x_0)$$

by [Claim 0.0.1](#) and we know $g_n \rightarrow 0$ uniformly. Hence, we know $(a_k)_{k=0}^\infty$ and $(b_k)_{k=0}^\infty$ converges to same point. Thus, $(S_n(x_0))_{n=1}^\infty$ converges. Note that this argument holds for all $x_0 \in T$, so we know $\lim_{n \rightarrow \infty} S_n$ exists.

Now since for all $\varepsilon > 0$, there exists $N > 0$ s.t. $n \geq N$ implies $g_{n+1}(x) = |g_{n+1}(x)| < \varepsilon$ for all $x \in T$, so $n \geq N$ implies

$$\begin{aligned} \left| \sum_{k=1}^n (-1)^{k+1} g_k(x) - \sum_{k=1}^\infty (-1)^{k+1} g_k(x) \right| &= \left| \sum_{k=n+1}^\infty (-1)^{k+1} g_k(x) \right| \\ &= \left| \lim_{m \rightarrow \infty} \sum_{k=n+1}^m (-1)^{k+1} g_k(x) \right| \\ &= \lim_{m \rightarrow \infty} \sum_{k=n+1}^m (-1)^{k+1} g_k(x) \\ &\leq \lim_{m \rightarrow \infty} g_{n+1}(x) = g_{n+1}(x) < \varepsilon \end{aligned}$$

for all $x \in T$ by [Claim 0.0.1](#) and [Claim 0.0.2](#), which means $\sum_{n=0}^\infty (-1)^{n+1} g_n(x)$ converges uniformly on T . \blacksquare

Problem 0.0.4 (15pts).

$$f_n(x) = \frac{x}{1 + nx^2}, \quad x \in \mathbb{R}, \quad n = 1, 2, \dots$$

Find the limit function f of the sequence $\{f_n\}$ and the limit function g of the sequence $\{f'_n\}$.

- Prove that $f'(x)$ exists for every x but that $f'(0) \neq g(0)$. For what values of x is $f'(x) = g(x)$?
- In what subintervals of \mathbb{R} does $f_n \rightarrow f$ uniformly?
- In what subintervals of \mathbb{R} does $f'_n \rightarrow g$ uniformly?

Problem 0.0.5 (15pts). Prove that

$$\sum x^n(1-x)$$

converges pointwise but not uniformly on $[0, 1]$, whereas

$$\sum (-1)^n x^n (1 - x)$$

converges uniformly on $[0, 1]$. This illustrates that uniform convergence of $\sum f_n(x)$ along with pointwise convergence of $\sum |f_n(x)|$ does not necessarily imply uniform convergence of $\sum |f_n(x)|$.

Proof. Suppose $S_N(x) = \sum_{n=0}^N x^n (1 - x)$, then we know

$$S_N(x) = (1 - x) \sum_{n=0}^N x^n = (1 - x) \frac{1 - x^{N+1}}{1 - x} = 1 - x^{N+1}.$$

Now suppose

$$f(x) = \begin{cases} 1, & \text{if } x \in [0, 1); \\ 0, & \text{if } x = 1. \end{cases}$$

Then, we claim that $\sum_{n=0}^{\infty} x^n (1 - x) \rightarrow f(x)$ pointwise on $[0, 1]$.

- Case 1: $x = 1$, then for all $\varepsilon > 0$, we can pick $N_1 = 1$ so that $n \geq N_1$ implies

$$|S_n(1) - f(1)| = |(1 - 1^{n+1}) - 0| = 0 < \varepsilon.$$

- Case 2: $x \in [0, 1)$, then for all $\varepsilon > 0$, we know there exists $N_2 > 0$ s.t. $x^{N_2+1} < \varepsilon$. Hence, $n \geq N_2$ implies

$$|S_n(x) - f(x)| = |1 - x^{n+1} - 1| = |x^{n+1}| = x^{n+1} \leq x^{N_2+1} < \varepsilon.$$

Hence, we're done. Now we show that $\sum_{n=0}^{\infty} x^n (1 - x)$ does not converge uniformly on $[0, 1]$. Suppose by contradiction, $\sum_{n=0}^{\infty} x^n (1 - x)$ converges uniformly to f , then for all $\varepsilon > 0$, there exists $N_3 > 0$ s.t. $n \geq N_3$ implies

$$|1 - x^{n+1} - f(x)| < \varepsilon \quad \forall x \in [0, 1].$$

Hence, if we pick some n_1, n_2 s.t. $n_1 > n_2 \geq N_3$, then we have

$$|1 - x^{n_1+1} - f(x)| < \varepsilon, \quad |1 - x^{n_2+1} - f(x)| < \varepsilon,$$

so by triangle inequality we have

$$\begin{aligned} |x^{n_2+1} - x^{n_1+1}| &= |1 - x^{n_1+1} - f(x) + (-1 + x^{n_2+1} + f(x))| \\ &\leq |1 - x^{n_1+1} - f(x)| + |1 - x^{n_2+1} - f(x)| < 2\varepsilon \end{aligned}$$

Note that

$$\begin{aligned} x^{n_2+1} (1 - x) &= x^{n_2+1} - x^{n_2+2} \leq x^{n_2+1} - x^{n_1+1} \\ &= |x^{n_2+1} - x^{n_1+1}| < 2\varepsilon. \end{aligned}$$

If we pick $x = 0.5$ and ε s.t. $0 < \varepsilon < \frac{0.5^{n_2+2}}{2}$, then we have

$$0.5^{n_2+2} < 2\varepsilon < 0.5^{n_2+2},$$

which is a contradiction. Hence, $\sum_{n=0}^{\infty} x^n (1 - x)$ does not converge uniformly.

Now we show that $\sum_{n=0}^{\infty} (-1)^n x^n (1 - x)$ converges uniformly on $[0, 1]$. Suppose

$$s_N(x) = \sum_{n=0}^N (-1)^n x^n (1 - x) = (1 - x) \sum_{n=0}^N (-x)^n = (1 - x) \frac{1 - (-x)^{N+1}}{1 - (-x)} = \frac{(1 - x)(1 - (-x)^{N+1})}{1 + x},$$

and $g(x) = \frac{1-x}{1+x}$, then we claim that $\sum_{n=0}^{\infty} (-1)^n x^n (1-x) \rightarrow g(x)$ uniformly on $[0, 1]$. Note that

$$|s_n(x) - g(x)| = \left| \frac{1-x}{1+x} (1 - (-x)^{n+1} - 1) \right| = \left| \frac{1-x}{1+x} x^{n+1} \right| \leq (1-x)x^{n+1}.$$

Suppose $h_n(x) = (1-x)x^{n+1} = x^{n+1} - x^{n+2}$, then

$$h'_n(x) = (n+1)x^n - (n+2)x^{n+1} = x^n((n+1) - (n+2)x),$$

so we know h_n attains its maximum on $[0, 1]$ at $x = \frac{n+1}{n+2}$. Hence, we have

$$\begin{aligned} |s_n(x) - g(x)| &\leq (1-x)x^{n+1} \leq \left(1 - \frac{n+1}{n+2}\right) \left(\frac{n+1}{n+2}\right)^{n+1} \\ &= \frac{1}{n+2} \left(1 - \frac{1}{n+2}\right)^{n+1} = \frac{1}{(n+2)} \frac{1}{\left(1 + \frac{1}{-(n+2)}\right)^{-(n+2)}} \\ &= \frac{1}{n+2} \frac{1}{\left(1 + \frac{1}{-(n+2)}\right)^{-(n+2)}} \rightarrow 0 \cdot \frac{1}{e} = 0 \text{ as } n \rightarrow \infty. \end{aligned}$$

Also, suppose

$$p(n) = \left(1 - \frac{n+1}{n+2}\right) \left(\frac{n+1}{n+2}\right)^{n+1} = \frac{(n+1)^{n+1}}{(n+2)^{n+2}},$$

for $n \geq 0$, then suppose

$$h(n) = \ln(p(n)) = (n+1)\ln(n+1) - (n+2)\ln(n+2),$$

we know

$$h'(n) = \ln(n+1) + 1 - \ln(n+2) - 1 = \ln\left(\frac{n+1}{n+2}\right) < 0,$$

which means $\ln(p(n))$ is decreasing when $n \geq 0$, which means $p(n)$ is decreasing when $n \geq 0$. Hence, for all $\varepsilon > 0$, we can pick some $N > 0$ s.t.

$$p(N) = \frac{(N+1)^{N+1}}{(N+2)^{N+2}} < \varepsilon,$$

and thus for all $n \geq N$ we have

$$|s_n(x) - g(x)| \leq p(n) \leq p(N) < \varepsilon \quad \forall x \in [0, 1],$$

which means $\sum_{n=0}^{\infty} (-1)^n x^n (1-x) \rightarrow g(x)$ uniformly on $[0, 1]$. ■

Problem 0.0.6 (15pts). Let

$$f_n(x) = \frac{1}{n} e^{-n^2 x^2}, \quad x \in \mathbb{R}, \quad n = 1, 2, \dots$$

Prove that $f_n \rightarrow 0$ uniformly on \mathbb{R} , that $f'_n \rightarrow 0$ pointwise on \mathbb{R} , but that the convergence of $\{f'_n\}$ is not uniform on any interval containing the origin.

Problem 0.0.7 (10pts). Let $\{f_n\}$ be a sequence of real-valued continuous functions defined on $[0, 1]$ and assume that $f_n \rightarrow f$ uniformly on $[0, 1]$. Prove or disprove

$$\lim_{n \rightarrow \infty} \int_0^{1-1/n} f_n(x) dx = \int_0^1 f(x) dx.$$

Proof. First note that

$$\int_0^1 f(x) dx = \int_0^1 \lim_{n \rightarrow \infty} f_n(x) dx = \lim_{n \rightarrow \infty} \int_0^1 f_n(x) dx$$

since $f_n \rightarrow f$ uniformly on $[0, 1]$. Also, since f_n is continuous and defined on $[0, 1]$ for all $n \in \mathbb{N}$, so by Extreme value theorem we know $f_n(x) \leq M$ for some $M \in \mathbb{R}$ for all $n \in \mathbb{N}$. Hence, we know

$$\int_0^1 f_n(x) dx - \int_0^{1-\frac{1}{n}} f_n(x) dx = \int_{1-\frac{1}{n}}^1 f_n(x) dx \leq M \cdot \frac{1}{n} \quad \forall n \in \mathbb{N}.$$

Hence, for all $\varepsilon > 0$ we can pick some $N > 0$ s.t. $M \cdot \frac{1}{N} < \varepsilon$ so that $n \geq N$ implies

$$\int_0^1 f_n(x) dx - \int_0^{1-\frac{1}{n}} f_n(x) dx \leq M \cdot \frac{1}{n} \leq M \cdot \frac{1}{N} < \varepsilon,$$

which means

$$\lim_{n \rightarrow \infty} \int_0^1 f_n(x) dx - \int_0^{1-\frac{1}{n}} f_n(x) dx = 0,$$

so

$$\lim_{n \rightarrow \infty} \int_0^1 f_n(x) dx = \lim_{n \rightarrow \infty} \int_0^{1-\frac{1}{n}} f_n(x) dx,$$

and thus

$$\int_0^1 f(x) dx = \lim_{n \rightarrow \infty} \int_0^1 f_n(x) dx = \lim_{n \rightarrow \infty} \int_0^{1-\frac{1}{n}} f_n(x) dx,$$

and we're done.

Remark 0.0.1. Since f_n is continuous and defined on $[0, 1]$, so f_n is Riemann integrable and thus f is Riemann integrable. Hence, we know

$$\int_0^1 f(x) dx = \lim_{n \rightarrow \infty} \int_0^1 f_n(x) dx$$

exists. Hence, we know

$$\begin{aligned} - \lim_{n \rightarrow \infty} \int_0^1 f_n(x) dx &= \lim_{n \rightarrow \infty} \int_0^1 f_n(x) dx - \int_0^{1-\frac{1}{n}} f_n(x) dx - \lim_{n \rightarrow \infty} \int_0^1 f_n(x) dx \\ &= \lim_{n \rightarrow \infty} \left(\int_0^1 f_n(x) dx - \int_0^{1-\frac{1}{n}} f_n(x) dx - \int_0^1 f_n(x) dx \right) \\ &= \lim_{n \rightarrow \infty} - \int_0^{1-\frac{1}{n}} f_n(x) dx \end{aligned}$$

exists. These are some details about why we can operate the limit as above.